progress on flow_upd

templates/flows/flow_upd.v
@@ -13,7 +13,7 @@ Section list_flow_upd.
   
   Definition edgeset (es: gmap Node (gmap Node (gset K))) n1 n2 : gset K :=
     (es !!! n1) !!! n2.
-  
+
   Definition find_next (esn: gmap Node (gset K)) (k: K) : option Node := 
     let f := λ (n': Node) (esn': gset K) res, 
               match res with
@@ -22,8 +22,15 @@ Section list_flow_upd.
                         then Some n'
                         else None end in
     map_fold f (None: option Node) esn.
-    
-  Function flow_upd_rec (es: gmap Node (gmap Node (gset K)))
+
+  Definition edge_rank_rel (es: gmap Node (gmap Node (gset K))) 
+    (rank: Node → nat) :=
+    ∀ n1 n2, edgeset es n1 n2 ≠ ∅ → rank n1 < rank n2. 
+
+  Definition outflow_edge_rel (n: Node) (esn: gmap Node (gset K)) In :=
+    ∀ n', outset K In n' = esn !!! n' ∩ inset K In n.
+
+  Function flow_updk_rec (es: gmap Node (gmap Node (gset K)))
     (I: gmap Node (multiset_flowint_ur K)) (k: K) 
     (n: Node) (R: gset Node)
     (I': gmap Node (multiset_flowint_ur K))
@@ -34,7 +41,7 @@ Section list_flow_upd.
     match find_next (es !!! n) k with
     | None => Some (I', n)
     | Some n1 => 
-      (* Have to pick from I' because its inflow is already updated *)
+      (* Have to pick from I' because n's inflow is already updated *)
       let In := I' !!! n in
       (* Add k to outf(In, n1) *)
       let In' := outflow_insert_set In n1 {[k]} in
@@ -44,34 +51,24 @@ Section list_flow_upd.
       let In1' := inflow_insert_set In1 n1 {[k]} in
       let II := <[n := In']> I' in
       let II' := <[n1 := In1']> II in  
-      flow_upd_rec es I k n1 (R ∖ {[n]}) II' end end.
+      flow_updk_rec es I k n1 (R ∖ {[n]}) II' end end.
   intros es I k n R I' Hbool n1 ?.
   rewrite bool_decide_eq_true in Hbool.
   assert (R ∖ {[n]} ⊂ R). 
   { set_solver. } by apply subset_size.
   Defined.
+  
+  Definition flow_updk_post (I II: gmap Node (multiset_flowint_ur K)) :=
+    let f := λ m1 m2,
+              match m1, m2 with 
+              | Some m1, Some m2 => Some m2
+              | None, Some m2 => Some m2
+              | Some m1, None => Some m1
+              | None, None => None end in
+    merge f I II.
+  
 
-(*
-  Fixpoint flow_upd_rec k (I I': gmap Node (multiset_flowint_ur K)) l :=
-    match l with
-    | [] => None
-    | [n] => Some (I', n)
-    | n :: (n1 :: ns) as nss =>
-      (* Have to pick from I' because its inflow is already updated *)
-      let In := I' !!! n in
-      (* Add k to outf(In, n1) *)
-      let In' := outflow_insert_set In n1 {[k]} in
-      (* Pick from I because n1 must be untouched so far *)
-      let In1 := I !!! n1 in
-      (* Add k to inf(In1, n1) *)
-      let In1' := inflow_insert_set In1 n1 {[k]} in
-      let II := <[n := In']> I' in
-      let II' := <[n1 := In1']> II in  
-      flow_upd_rec k I II' nss end.
-        
-  Functional Scheme flow_upd_rec_ind := Induction for flow_upd_rec Sort Prop.
-    
-  Definition flow_upd S es n0 (k: K) I : option (gmap Node (multiset_flowint_ur K) * Node) :=
+  Definition flow_updk es I k n0 :=
     match find_next (es !!! n0) k with
     | None => None
     | Some n1 =>
@@ -79,72 +76,253 @@ Section list_flow_upd.
       let In0' := outflow_insert_set In0 n1 {[k]} in
       let In1 := I !!! n1 in
       let In1' := inflow_insert_set In1 n1 {[k]} in
-      let I' := <[n1 := In1']> {[n0 := In0']} in
-      match prepare_upd S es n1 k with
-      | None => None
-      | Some l => 
-        flow_upd_rec k I I' l end end.  
-*)
+      let I' := <[n1 := In1']> ({[n0 := In0']}) in
+      match flow_updk_rec es I k n1 (dom I ∖ {[n0]}) I' with
+      | Some (II, nk) =>
+        let II' := flow_updk_post I II in
+        Some (II', nk)
+      | None => None end end.
 
-  Lemma flow_upd_intfEq es I k n R I' II' nl:
+    
+  Lemma flow_upd_defined rank es I k n R I':
+    (edge_rank_rel es rank) →
+    (∀ n1 n2, edgeset es n1 n2 ≠ ∅ → n2 ∈ dom I) →
+    (n ∈ dom I') →
+    (dom I = R ∪ dom I') →
+    (R ∩ dom I' = {[n]}) →
+    (∀ x, x ∈ dom I' → rank x ≤ rank n) →
+      flow_updk_rec es I k n R I' ≠ None.
+  Proof.
+  (*
+    apply flow_updk_rec_ind; try done.
+    - clear n R. intros n R I0 n_notin_R.
+      rewrite bool_decide_eq_false in n_notin_R.
+      intros _ _ _ _ ? _; set_solver.
+    - clear n R. intros n R I0 n_in_R.
+      rewrite bool_decide_eq_true in n_in_R.
+      intros n1 FN_n In In' In1 In1' II I0' HInd EdgeRank
+        ES_I n_in_I0 Dom_I R_inter_I0 Rank_I0.
+      assert (edgeset es n n1 ≠ ∅) as ES_n_n1. { admit. }
+      assert (n1 ∉ dom I0) as n1_notin_I0.
+      { pose proof EdgeRank n n1 ES_n_n1 as H'.
+        intros n1_in_I0. apply Rank_I0 in n1_in_I0.
+        clear -H' n1_in_I0. lia. }
+      assert (dom I0' = dom I0 ∪ {[n1]}) as Dom_I0'.
+      { rewrite /I0' /II.
+        repeat rewrite dom_insert_L.
+        clear -n_in_I0 n1_notin_I0.
+        set_solver. }
+      assert (n1 ∈ dom I) as n1_in_I.
+      { by pose proof ES_I n n1 ES_n_n1. }  
+      assert (n1 ∈ R) as n1_in_R.
+      { rewrite Dom_I in n1_in_I. 
+        clear -n1_notin_I0 n1_in_I. 
+        set_solver. }
+      apply HInd; try done.
+      + rewrite Dom_I0'; clear; set_solver.
+      + rewrite Dom_I Dom_I0'.
+        clear -n_in_I0 n1_in_R R_inter_I0.
+        assert (R ∖ {[n]} ∪ (dom I0 ∪ {[n1]}) ⊆ R ∪ dom I0) as H'.
+        { set_solver. }
+        assert (R ∪ dom I0 ⊆ R ∖ {[n]} ∪ (dom I0 ∪ {[n1]})) as H''.
+        { intros x; rewrite elem_of_union.
+          intros [Hx|Hx]; last first.
+          - set_solver.
+          - destruct (decide (x = n)) as [-> | Hxn]. 
+            + set_solver.
+            + set_solver. }
+        clear -H' H''; set_solver.
+      + rewrite Dom_I0'.
+        clear -n1_in_R R_inter_I0 n1_notin_I0. set_solver. 
+      + pose proof EdgeRank n n1 ES_n_n1 as H'. 
+        rewrite Dom_I0'. intros x; rewrite elem_of_union.
+        intros [Hx | Hx].
+        * apply Rank_I0 in Hx. clear -Hx H'. lia.
+        * assert (x = n1) as -> by (clear -Hx; set_solver).
+          clear; lia.
+  *)
+  Admitted.
+      
+      
+      
+
+  Lemma flow_updk_invariants rank es I k n R I' II' nk n0:
     let FI := λ I x, I !!! x in 
-      (* (NoDup l) →
-      (match l with 
-        | [] => True 
-        | n :: ns => 
-            n ∈ dom I'
-          ∧ FI I' n = inflow_insert_set (FI I n) n {[k]}
-          ∧ (list_to_set ns ## dom I') end) → *)
-      (n ∈ dom I') →
-      (FI I' n = inflow_insert_set (FI I n) n {[k]}) →
+      (edge_rank_rel es rank) →
       (✓ ([^op set] x ∈ dom I, FI I x)) →
-      (dom I' ⊆ dom I) →
-      (* (list_to_set l ⊆ dom I) → *)
       (∀ x, x ∈ dom I → domm (FI I x) = {[x]}) →
+      (∀ n1 n2, edgeset es n1 n2 ≠ ∅ → n2 ∈ dom I) →
+      (∀ x, x ∈ dom I → outflow_edge_rel x (es !!! x) (FI I x)) →
+      (∀ x, x ∈ dom I' ∖ {[n]} → outflow_edge_rel x (es !!! x) (FI I' x)) →
+      (n0 ∈ dom I') → (n ∈ dom I') → (n0 ≠ n) →
+      (∀ x, x ∈ dom I' → rank x ≤ rank n) →
+      (∀ x, x ∈ dom I' ∖ {[n0]} → rank n0 < rank x) →
+      (FI I' n = inflow_insert_set (FI I n) n {[k]}) →
+      (dom I' ⊆ dom I) →
+      (∀ x, x ∈ dom I' ∖ {[n0; n]} → keyset (FI I' x) = keyset (FI I x)) →
+      (keyset (FI I' n0) = keyset (FI I n0) ∖ {[k]}) →
+      (k ∈ insets (FI I n)) →
       (∀ x, x ∈ dom I' → domm (FI I' x) = {[x]}) →
       ([^op set] x ∈ dom I', FI I x) = ([^op set] x ∈ dom I', FI I' x) →
-        flow_upd_rec es I k n R I' = Some (II', nl) → 
-          (([^op set] x ∈ dom II', FI I x) = ([^op set] x ∈ dom II', FI II' x)
-          ∧ keyset (FI II' nl) = keyset (FI I nl) ∪ {[k]}).
+      flow_updk_rec es I k n R I' = Some (II', nk) →
+          ((([^op set] x ∈ dom II', FI I x) = ([^op set] x ∈ dom II', FI II' x))
+          ∧ (keyset (FI II' nk) = keyset (FI I nk) ∪ {[k]})
+          ∧ (keyset (FI II' n0) = keyset (FI I n0) ∖ {[k]})
+          ∧ (∀ x, x ∈ dom II' ∖ {[n0; nk]} → keyset (FI II' x) = keyset (FI I x))
+          ∧ (∀ x, x ∈ dom II' → outflow_edge_rel x (es !!! x) (FI II' x))
+          ∧ (dom II' ⊆ dom I)
+          ∧ (n0 ≠ nk)
+          ∧ (n0 ∈ dom II')
+          ∧ (nk ∈ dom II')
+          ∧ (∀ x, x ∈ dom II' → domm (FI II' x) = {[x]})).
   Proof.
-    intros FI. apply flow_upd_rec_ind.
+  (*
+    intros FI. apply flow_updk_rec_ind.
     - intros; try done.
-    - intros n0 R0 I0 n0_in_R0 FN_n0 n0_in_I0 Def_I0_n0 VI Dom_I0_in_I 
-        Domm_I Domm_I0 Heq [= -> ->]. split; try done. rewrite Def_I0_n0.
-      rewrite /keyset. rewrite inflow_insert_set_insets.
-      rewrite inflow_insert_set_outsets.
-      assert (k ∉ outsets (FI I nl)) as H'.
-      { admit. }
-      clear -H'; set_solver.
-    - intros n0 R0 I0 n0_in_R0 n1 FN_n0.
-      intros In In' In1 In1' II I0' HInd n_in_I0 Def_I0_n0 
-        VI Dom_I0_in_I Domm_I Domm_I0 Heq Hflow.
+    - clear n R. intros n R I0 n_in_R FN_n EdgeRank VI Domm_I ES_I 
+        Outflow_I Outflow_I0 n0_in_I0 n_in_I0 n0_neq_n Rank_I0 Rank_n0 
+        Def_I0_n Dom_I0_in_I KS_I0 KS_n0 k_in_Insn Domm_I0 Heq [= -> ->]. 
+      repeat split; try done.
+      + rewrite Def_I0_n.
+        rewrite /keyset. rewrite inflow_insert_set_insets.
+        rewrite inflow_insert_set_outsets.
+        assert (k ∉ outsets (FI I nk)) as H'.
+        { admit. }
+        clear -H'; set_solver.
+      + intros x Hx. destruct (decide (x = nk)) as [-> | Hxn].
+        * intros n'. rewrite Def_I0_n.
+          rewrite inflow_insert_set_outset_ne.
+          rewrite inflow_insert_set_inset.
+          assert (nk ∈ dom I) as H' by (clear -Hx Dom_I0_in_I; set_solver).
+          pose proof Outflow_I nk H' n' as H''.
+          assert (k ∉ (es !!! nk) !!! n') as Hk.
+          { admit. }
+          assert (k ∉ outset K (FI I nk) n') as H'''.
+          { clear -H'' Hk. set_solver. }
+          clear -Hk H'' H'''; set_solver.
+        * assert (x ∈ dom II' ∖ {[nk]}) as Hx' by set_solver.
+          by apply Outflow_I0.      
+    - clear n R. intros n R I0 n_in_R n1 FN_n.
+      intros In In' In1 In1' II I0' HInd EdgeRank VI Domm_I ES_I Outflow_I 
+        Outflow_I0 n0_in_I0 n_in_I0 n0_neq_n Rank_I0 Rank_n0 Def_I0_n 
+        Dom_I0_in_I KS_I0 KS_n0 k_in_Insn Domm_I0 Heq Hflow.
+      assert (edgeset es n n1 ≠ ∅) as ES_n_n1. { admit. }
       assert (n1 ∉ dom I0) as n1_notin_I0.
-      { clear -HdomI_disj. set_solver. }
+      { pose proof EdgeRank n n1 ES_n_n1 as H'.
+        intros n1_in_I0. apply Rank_I0 in n1_in_I0.
+        clear -H' n1_in_I0. lia. }
       assert (dom I0' = dom I0 ∪ {[ n1 ]}) as Dom_I0'.
       { rewrite /I0' /II.
         repeat rewrite dom_insert_L.
         clear -n_in_I0 n1_notin_I0.
         set_solver. }
       assert (n1 ∈ dom I) as n1_in_I.
-      { clear -l_in_I. set_solver. }  
-      assert (∀ x, x ∈ dom I0 → domm (FI (<[n:=In']> I0) x) = {[x]}) as Domm_II.
+      { by pose proof ES_I n n1 ES_n_n1. }  
+      assert (∀ x, x ∈ dom I0 → domm (FI (<[n:=In']> I0) x) = {[x]}) 
+        as Domm_II.
       { intros x Hx. destruct (decide (n = x)) as [-> | Hxn].
         - unfold FI. rewrite lookup_total_insert.
           subst In'. rewrite flowint_outflow_map_set_domm.
           subst In. rewrite Domm_I0; try done.
         - unfold FI. rewrite lookup_total_insert_ne; try done.
           rewrite Domm_I0; try done. }
+      assert (n0 ≠ n1) as n0_neq_n1.
+      { clear -n0_in_I0 n1_notin_I0. set_solver. }    
       apply HInd; try done; clear HInd.
-      { clear -NoDup. apply NoDup_cons in NoDup.
-        destruct NoDup as [_ ?]; try done. }
-      { rewrite Dom_I0'. split. 
-        - clear; set_solver.
-        - apply NoDup_cons in NoDup. destruct NoDup as [_ NoDup]. 
-          apply NoDup_cons in NoDup. destruct NoDup as [NoDup _].
-          clear -HdomI_disj NoDup. set_solver. }
+      { rewrite /FI. rewrite Dom_I0'. intros x; rewrite elem_of_difference.
+        intros [Hx1 Hx2]. rewrite elem_of_union in Hx1.
+        destruct Hx1 as [Hx | Hx].
+        - rewrite /I0'. 
+          assert (x ≠ n1) by (clear -Hx n1_notin_I0; set_solver).
+          rewrite lookup_total_insert_ne; try done. rewrite /II.
+          destruct (decide (x = n)) as [-> | Hxn].
+          + rewrite lookup_total_insert. subst In'.
+            unfold outflow_edge_rel. intros n'.
+            rewrite outflow_insert_set_inset.
+            assert (n ∈ dom I) as H' by 
+              (clear -n_in_I0 Dom_I0_in_I; set_solver).
+            destruct (decide (n' = n1)) as [-> | Hn'n].
+            * rewrite outflow_insert_set_outset.
+              rewrite /In.
+              pose proof Outflow_I n H' n1 as H''.
+              unfold FI in Def_I0_n. rewrite Def_I0_n.
+              rewrite inflow_insert_set_outset_ne.
+              rewrite inflow_insert_set_inset.
+              unfold FI in H''.
+              assert (k ∈ (es !!! n) !!! n1) as Hk.
+              { admit. }
+              clear -Hk H''. set_solver.
+            * rewrite outflow_insert_set_outset_ne; try done.
+              rewrite /In.
+              pose proof Outflow_I n H' n' as H''.
+              rewrite /FI in H''. rewrite /FI in Def_I0_n.
+              rewrite Def_I0_n.
+              rewrite inflow_insert_set_outset_ne.
+              rewrite inflow_insert_set_inset.
+              assert (k ∉ (es !!! n) !!! n') as Hk.
+              { admit. }
+              assert (k ∉ outset K (FI I n) n') as H'''.
+              { clear -H'' Hk. set_solver. }
+              clear -Hk H''. set_solver.
+          + rewrite lookup_total_insert_ne; try done.
+            apply Outflow_I0. clear -Hx Hxn; set_solver.
+        - clear -Hx Hx2; set_solver. }
+      { rewrite Dom_I0'. clear -n0_in_I0.
+        set_solver. }
       { rewrite Dom_I0'. clear -Dom_I0_in_I n1_in_I. set_solver. }
-      { clear -l_in_I. set_solver. }
+      { pose proof EdgeRank n n1 ES_n_n1 as H'. 
+        rewrite Dom_I0'. intros x; rewrite elem_of_union.
+        intros [Hx | Hx].
+        - apply Rank_I0 in Hx. clear -Hx H'. lia.
+        - assert (x = n1) as -> by (clear -Hx; set_solver).
+          clear; lia. }
+      { rewrite Dom_I0'. intros x. rewrite elem_of_difference.
+        rewrite elem_of_union. intros [[Hx1 | Hx1] Hx2].
+        - apply Rank_n0. clear -Hx1 Hx2; set_solver.
+        - assert (x = n1) as -> by (clear -Hx1; set_solver). 
+          pose proof EdgeRank n n1 ES_n_n1 as H'.
+          assert (rank n0 ≤ rank n) as H''.
+          { by apply Rank_I0. }
+          clear -H' H''. lia. }    
+      { rewrite /I0' /FI. rewrite lookup_total_insert. 
+        rewrite /In1'. by rewrite /In1. }
+      { rewrite Dom_I0'. intros x; rewrite elem_of_union.
+        intros [Hx | Hx].
+        - by apply Dom_I0_in_I.
+        - assert (x = n1) as -> by (clear -Hx; set_solver).
+          clear -n1_in_I; set_solver. }
+      { intros x. rewrite Dom_I0'. rewrite elem_of_difference.
+        rewrite elem_of_union. intros [[Hx1 | Hx1] Hx2].
+        - destruct (decide (x = n)) as [-> | Hxn].
+          + unfold FI. subst I0'.
+            rewrite lookup_total_insert_ne; 
+              last by (clear -Hx2; set_solver).
+            subst II. rewrite lookup_total_insert.
+            subst In'. unfold keyset.
+            rewrite outflow_insert_set_insets.
+            rewrite outflow_insert_set_outsets.
+            subst In. unfold FI in Def_I0_n. rewrite Def_I0_n.
+            rewrite inflow_insert_set_insets.
+            rewrite inflow_insert_set_outsets.
+            unfold FI in k_in_Insn.
+            assert (k ∈ outsets (I !!! n)) as H'.
+            { admit. } 
+            clear -k_in_Insn H'; set_solver.
+          + unfold FI. subst I0'.
+            rewrite lookup_total_insert_ne; 
+              last by (clear -Hx2; set_solver).
+            subst II. rewrite lookup_total_insert_ne; try done.
+            apply KS_I0. clear -Hx1 Hx2 Hxn; set_solver.
+        - clear -Hx1 Hx2; set_solver. }
+      { subst I0'. unfold FI. 
+        rewrite lookup_total_insert_ne; try done.
+        subst II. rewrite lookup_total_insert_ne; try done.  }  
+      { assert (k ∈ inset K (FI I n1) n1) as H'. 
+        { apply (flowint_inset_step (FI I n) _ _ _).
+          - admit.
+          - rewrite Domm_I; try done. clear; set_solver.
+          - admit. }
+        admit. }    
       { rewrite Dom_I0'. intros x; rewrite elem_of_union.
         intros [Hx | Hx].
         - subst I0'. 
@@ -161,7 +339,8 @@ Section list_flow_upd.
           rewrite flowint_inflow_map_set_dom.
           subst In1. rewrite Domm_I; try done.
           clear; set_solver. }
-      rewrite Dom_I0'. rewrite !big_opS_union; [try done | set_solver | set_solver].
+      rewrite Dom_I0'. 
+      rewrite !big_opS_union; [try done | set_solver | set_solver].
       rewrite !big_opS_singleton. 
       all: try (clear -n_notin_I0; set_solver).
       rewrite /I0'; rewrite /FI. rewrite lookup_total_insert.
@@ -244,15 +423,19 @@ Section list_flow_upd.
         - rewrite Domm_II_eq_I. try done. 
         - intros n'. unfold inf. rewrite outflow_map_set_inf.
           assert (inf ([^op set] y ∈ dom I0, FI (<[n:=In']> I0) y) n'
-            ≡ default 0 (inf_map ([^op set] y ∈ dom I0, FI (<[n:=In']> I0) y) !! n'))
+            ≡ default 0 
+              (inf_map ([^op set] y ∈ dom I0, FI (<[n:=In']> I0) y) !! n'))
             as HL by try done.
           assert (inf ([^op set] y ∈ dom I0, FI I y) n'
-            ≡ default 0 (inf_map ([^op set] y ∈ dom I0, I !!! y) !! n')) as HR by try done.
+            ≡ default 0 
+              (inf_map ([^op set] y ∈ dom I0, I !!! y) !! n')) 
+            as HR by try done.
           rewrite <-HL. rewrite <-HR.
           rewrite Heq.
           assert (inf ([^op set] y ∈ dom I0, FI (<[n:=In']> I0) y) n' = 
                     inf ([^op set] y ∈ dom I0, FI I0 y) n') as HI0.
-          { destruct (decide (n' ∈ domm ([^op set] y ∈ dom I0, FI (<[n:=In']> I0) y))) 
+          { destruct (decide (n' ∈ 
+                        domm ([^op set] y ∈ dom I0, FI (<[n:=In']> I0) y))) 
               as [Hn' | Hn'].
             - rewrite flow_big_op_dom in Hn'; try done.
               destruct Hn' as [n'' [n''_in_I0 n'_in_n'']].
@@ -261,43 +444,54 @@ Section list_flow_upd.
               rewrite (flow_big_op_inf _ _ n'); try done.
               + rewrite (flow_big_op_inf _ _ n'); try done.
                 * clear HL HR. 
-                  assert (([^+ set] x ∈ (dom I0 ∖ {[n']}), out (FI (<[n:=In']> I0) x) n')
-                    = ([^+ set] x ∈ (dom I0 ∖ {[n']}), out (FI I0 x) n')) as Hout.
+                  assert (([^+ set] x ∈ (dom I0 ∖ {[n']}), 
+                            out (FI (<[n:=In']> I0) x) n')
+                          = ([^+ set] x ∈ (dom I0 ∖ {[n']}), 
+                            out (FI I0 x) n')) as Hout.
                   { destruct (decide (n' = n)) as [-> | Hn'].
-                    - (* forall x ∈ dom I0 ∖ {[n]}, FI (<[n:=In']> I0) x = FI I0 x *)
+                    - (* forall x ∈ dom I0 ∖ {[n]}, 
+                            FI (<[n:=In']> I0) x = FI I0 x *)
                       (* syntactic rewriting *)
                       admit.
-                    - assert (out (FI (<[n := In']> I0) n) n' = out (FI I0 n) n') as H'.
+                    - assert (out (FI (<[n := In']> I0) n) n' 
+                                = out (FI I0 n) n') as H'.
                       { rewrite /FI. rewrite lookup_total_insert.
                         rewrite /In' /In.
-                        assert (n' ≠ n1). { clear -n''_in_I0 n1_notin_I0. set_solver. }
-                        unfold out. rewrite outflow_map_set_out_map_ne; try done. }
+                        assert (n' ≠ n1). 
+                        { clear -n''_in_I0 n1_notin_I0. set_solver. }
+                        unfold out. 
+                        rewrite outflow_map_set_out_map_ne; try done. }
                       (* break the big sum *)
                       (* syntactic rewriting + above assert *)
                       admit. }
-                  assert (inf (FI (<[n:=In']> I0) n') n' = inf (FI I0 n') n') as Hin.
+                  assert (inf (FI (<[n:=In']> I0) n') n' 
+                            = inf (FI I0 n') n') as Hin.
                   { destruct (decide (n' = n)) as [-> | Hn'].
-                    - rewrite /FI. rewrite lookup_total_insert. subst In'.
-                      unfold inf. rewrite outflow_map_set_inf. by subst In.
-                    - rewrite /FI. rewrite lookup_total_insert_ne; try done. }
+                    - rewrite /FI. rewrite lookup_total_insert. 
+                      subst In'. unfold inf. 
+                      rewrite outflow_map_set_inf. by subst In.
+                    - rewrite /FI. 
+                      rewrite lookup_total_insert_ne; try done. }
                   by rewrite Hin Hout.
                 * rewrite Domm_I0; try done.
               + rewrite Domm_II; try done.
             - (* syntactic rewriting + flow_inf lemma *) admit.
           }
           by rewrite HI0.
-        - rewrite Heq.
-          intros n'.
-          destruct (decide (n' ∈ domm ([^op set] y ∈ dom I0, FI (<[n:=In']> I0) y))) 
+        - rewrite Heq. intros n'.
+          destruct (decide (n' ∈ 
+              domm ([^op set] y ∈ dom I0, FI (<[n:=In']> I0) y))) 
               as [Hn' | Hn'].
           + (* syntactic rewriting + flow_outf lemma *) admit.     
           + destruct (decide (n' = n1)) as [-> | Hn1'].
-            * apply nzmap_eq. intros k'. destruct (decide (k' ∈ ({[k]}: gset K))) as [Hk' | Hk'].
+            * apply nzmap_eq. intros k'. 
+              destruct (decide (k' ∈ ({[k]}: gset K))) as [Hk' | Hk'].
               ** rewrite outflow_lookup_total_map_set; try done.
                  rewrite !flow_big_op_out.
                  (* break the big sum + lookup_total_lifting *)
                  admit.
-                 { apply leibniz_equiv_iff in Heq. rewrite <-Heq. try done. }
+                 { apply leibniz_equiv_iff in Heq. 
+                   rewrite <-Heq. try done. }
                  { intros Hn1. rewrite flow_big_op_dom in Hn1; try done.
                    destruct Hn1 as [x [Hx1 Hx2]].
                    rewrite Domm_I0 in Hx2; try done.
@@ -332,6 +526,366 @@ Section list_flow_upd.
       { rewrite /In1' /In1. try done. }
       assert (✓ (([^op set] y ∈ dom I0, FI I y) ⋅ (FI I n1))) as H0'''.
       {  admit. }
-      by pose proof Hpose n1_in_In1 Domm_I0_notEmpty H0' H0'' H0''' as Hpose.
-  Admitted.      
+      by pose proof Hpose n1_in_In1 Domm_I0_notEmpty H0' H0'' H0''' 
+        as Hpose.
+  *)      
+  Admitted.
+  
+  Lemma flow_updk_post_dom I II I' :
+    (dom II ⊆ dom I) →
+    I' = flow_updk_post I II →
+      dom I' = dom I.
+  Proof.
+    intros Hdom Hflow.
+    assert (dom I' ⊆ dom I).
+    { intros x. rewrite elem_of_dom.
+      subst I'. intros [m Hx].
+      unfold flow_updk_post in Hx.
+      rewrite lookup_merge in Hx.
+      unfold diag_None in Hx.
+      destruct (I !! x) as [mI |] eqn: HIx.
+      - rewrite elem_of_dom; try done.
+      - destruct (II !! x) as [mII |] eqn: HIIx; try done.
+        apply Hdom. rewrite elem_of_dom; try done. }
+    assert (dom I ⊆ dom I').
+    { intros x. rewrite !elem_of_dom.
+      intros [mx Hx]. subst I'.
+      unfold flow_updk_post.
+      rewrite lookup_merge.
+      unfold diag_None.
+      rewrite Hx.
+      destruct (II !! x) as [mII |]; try done. }
+    set_solver.      
+  Qed.          
+
+  Lemma flow_updk_post_intfEq I II I' :
+    let FI := λ I x, I !!! x in
+    (dom II ⊆ dom I) →
+    (([^op set] x ∈ dom II, FI I x) = ([^op set] x ∈ dom II, FI II x)) → 
+    I' = flow_updk_post I II →
+      (([^op set] x ∈ dom I, FI I x) = ([^op set] x ∈ dom I, FI I' x)).
+  Proof.
+  Admitted.
+
+  Lemma flow_updk_post_lookup I II I' :
+    (dom II ⊆ dom I) →
+    I' = flow_updk_post I II →
+      (∀ x, x ∈ dom II → I' !! x = II !! x).
+  Proof.
+    intros Dom_II_in_I Hflow. intros x Hx.
+    rewrite Hflow. unfold flow_updk_post.
+    rewrite lookup_merge. unfold diag_None.
+    destruct (I !! x) as [mI |] eqn: HmI.
+    - destruct (II !! x) as [mII |] eqn: HmII; try done.
+      apply not_elem_of_dom_2 in HmII.
+      set_solver.
+    - assert (II !! x = None) as H'.
+      { apply not_elem_of_dom. 
+        apply not_elem_of_dom_2 in HmI.
+        set_solver. }
+      by rewrite H'.
+  Qed.    
+
+  Lemma flow_updk_post_lookup_total I II I' :
+    (dom II ⊆ dom I) →
+    I' = flow_updk_post I II →
+      (∀ x, x ∈ dom II → I' !!! x = II !!! x).
+  Proof.
+    intros ? H' ? ?; rewrite !lookup_total_alt.
+    rewrite (flow_updk_post_lookup _ _ _ _ H'); try done.
+  Qed.  
+
+  Lemma flow_updk_post_lookup_ne I II I' :
+    (dom II ⊆ dom I) →
+    I' = flow_updk_post I II →
+      (∀ x, x ∈ dom I ∖ dom II → I' !! x = I !! x).
+  Proof.
+    intros Dom_II_in_I Hflow. intros x Hx.
+    rewrite elem_of_difference in Hx.
+    destruct Hx as [Hx1 Hx2].
+    rewrite Hflow. unfold flow_updk_post.
+    rewrite lookup_merge. unfold diag_None.
+    rewrite elem_of_dom in Hx1.
+    destruct Hx1 as [mI Hx1].
+    rewrite Hx1.
+    rewrite not_elem_of_dom in Hx2.
+    by rewrite Hx2.
+  Qed.  
+
+  Lemma flow_updk_post_lookup_total_ne I II I' :
+    (dom II ⊆ dom I) →
+    I' = flow_updk_post I II →
+      (∀ x, x ∈ dom I ∖ dom II → I' !!! x = I !!! x).
+  Proof.
+    intros ? H' ? ?; rewrite !lookup_total_alt.
+    rewrite (flow_updk_post_lookup_ne _ _ _ _ H'); try done.
+  Qed.
+  
+  Lemma flow_updk_post_summary (es: gmap Node (gmap Node (gset K)))
+    (k: K) (I II I': gmap Node (multiset_flowint_ur K))  
+    (n0 nk: Node) :
+    let FI := λ I x, I !!! x in
+    (dom II ⊆ dom I) →
+    (n0 ∈ dom II) → (nk ∈ dom II) →
+    (∀ x, x ∈ dom I → domm (FI I x) = {[x]}) →
+    (∀ x, x ∈ dom II → domm (FI II x) = {[x]}) →
+    (([^op set] x ∈ dom II, FI I x) = ([^op set] x ∈ dom II, FI II x)) → 
+    (keyset (FI II nk) = keyset (FI I nk) ∪ {[k]}) →
+    (keyset (FI II n0) = keyset (FI I n0) ∖ {[k]}) →
+    (∀ x, x ∈ dom II ∖ {[n0; nk]} → keyset (FI II x) = keyset (FI I x)) →
+    (∀ x, x ∈ dom I → outflow_edge_rel x (es !!! x) (FI I x)) →
+    (∀ x, x ∈ dom II → outflow_edge_rel x (es !!! x) (FI II x)) →
+    I' = flow_updk_post I II →
+          ((dom I' = dom I)
+        ∧ (∀ x, x ∈ dom I' → domm (FI I' x) = {[x]})  
+        ∧ (([^op set] x ∈ dom I, FI I x) = ([^op set] x ∈ dom I, FI I' x))
+        ∧ (keyset (FI I' nk) = keyset (FI I nk) ∪ {[k]})
+        ∧ (keyset (FI I' n0) = keyset (FI I n0) ∖ {[k]})
+        ∧ (∀ x, x ∈ dom I ∖ {[n0; nk]} → keyset (FI I' x) = keyset (FI I x))
+        ∧ (∀ x, x ∈ dom I → outflow_edge_rel x (es !!! x) (FI I' x))).
+  Proof.
+    intros FI Dom_II_in_I n0_in_II nk_in_II Domm_I Domm_II Heq 
+      KS_nk KS_n0 KS_II Outflow_I Outflow_II Hflow.
+    pose proof flow_updk_post_dom I II I' Dom_II_in_I Hflow as Dom_I'_eq_I.
+    pose proof flow_updk_post_intfEq I II I' Dom_II_in_I Heq Hflow as Heq'.
+    repeat split; try done.
+    - intros x Hx.  
+      destruct (decide (x ∈ dom II)) as [Hx1 | Hx1].
+      + unfold FI.
+        rewrite (flow_updk_post_lookup_total _ _ _ _ Hflow); try done.
+        apply Domm_II; try done.
+      + unfold FI.
+        rewrite (flow_updk_post_lookup_total_ne _ _ _ _ Hflow); try done.
+        apply Domm_I; try done.
+        all: clear -Dom_I'_eq_I Hx1 Hx; set_solver.
+    - assert (FI I' nk = FI II nk) as H'.
+      { unfold FI.
+        by rewrite (flow_updk_post_lookup_total _ _ _ _ Hflow). }
+      rewrite H'; try done.
+    - assert (FI I' n0 = FI II n0) as H'.
+      { unfold FI. 
+        by rewrite (flow_updk_post_lookup_total _ _ _ _ Hflow). }
+      rewrite H'; try done.
+    - intros x. rewrite elem_of_difference.
+      intros [Hx1 Hx2].
+      destruct (decide (x ∈ dom II)) as [Hx3 | Hx3].
+      + unfold FI.
+        rewrite (flow_updk_post_lookup_total _ _ _ _ Hflow); try done.
+        apply KS_II. clear -Hx3 Hx2; set_solver.
+      + unfold FI.
+        rewrite (flow_updk_post_lookup_total_ne _ _ _ _ Hflow); try done.
+        clear -Hx1 Hx3; set_solver.
+    - intros x Hx.  
+      destruct (decide (x ∈ dom II)) as [Hx1 | Hx1].
+      + unfold FI.
+        rewrite (flow_updk_post_lookup_total _ _ _ _ Hflow); try done.
+        apply Outflow_II; try done.
+      + unfold FI.
+        rewrite (flow_updk_post_lookup_total_ne _ _ _ _ Hflow); try done.
+        apply Outflow_I; try done.
+        clear -Hx1 Hx; set_solver.
+  Qed.
+
+  Lemma flow_updk_summary rank es I k n0 res:
+    let FI := λ I x, I !!! x in 
+    (edge_rank_rel es rank) →
+    (∀ n1 n2, edgeset es n1 n2 ≠ ∅ → n2 ∈ dom I) →
+    (✓ ([^op set] x ∈ dom I, FI I x)) →
+    (∀ x, x ∈ dom I → domm (FI I x) = {[x]}) →
+    (∀ x, x ∈ dom I → outflow_edge_rel x (es !!! x) (FI I x)) →
+    (n0 ∈ dom I) →
+    (find_next (es !!! n0) k ≠ None) →
+    flow_updk es I k n0 = res →
+      ∃ II' nk, 
+        res = Some (II', nk)
+      ∧ (dom II' = dom I)
+      ∧ (n0 ≠ nk)
+      ∧ (∀ x, x ∈ dom II' → domm (FI II' x) = {[x]})
+      ∧ (([^op set] x ∈ dom I, FI I x) = ([^op set] x ∈ dom I, FI II' x))
+      ∧ (keyset (FI II' nk) = keyset (FI I nk) ∪ {[k]})
+      ∧ (keyset (FI II' n0) = keyset (FI I n0) ∖ {[k]})
+      ∧ (∀ x, x ∈ dom I ∖ {[n0; nk]} → keyset (FI II' x) = keyset (FI I x))
+      ∧ (∀ x, x ∈ dom I → outflow_edge_rel x (es !!! x) (FI II' x)).
+  Proof.
+    intros FI EdgeRank ES_I VI Domm_I Outflow_I n0_in_I FN_n0 Hflow_upd.
+    unfold flow_updk in Hflow_upd.
+    destruct (find_next (es !!! n0) k) as [n1 |]; try done.
+    set In1 := inflow_insert_set (I !!! n1) n1 {[k]}.
+    set In0 := outflow_insert_set (I !!! n0) n1 {[k]}.
+    set I': gmap Node (multiset_flowint_ur K) := {[n1 := In1; n0 := In0]}.
+    assert (In1 = inflow_insert_set (I !!! n1) n1 {[k]}) as Def_In1.
+    { try done. }
+    assert (In0 = outflow_insert_set (I !!! n0) n1 {[k]}) as Def_In0.
+    { try done. }
+    assert (I' = {[n1 := In1; n0 := In0]}) as Def_I'.
+    { try done. }
+    rewrite <-Def_In1 in Hflow_upd.
+    rewrite <-Def_In0 in Hflow_upd.
+    rewrite <-Def_I' in Hflow_upd.
+    assert (dom I' = {[n0; n1]}) as Dom_I' by set_solver.
+    assert (n1 ∈ dom I') as n1_in_I' by set_solver.
+    assert (n1 ∈ dom I) as n1_in_I.
+    { apply (ES_I n0). admit. }
+    assert (n0 ≠ n1) as n0_neq_n1.
+    { admit. }
+    assert (dom I = (dom I ∖ {[n0]}) ∪ dom I') as H'.
+    { rewrite Dom_I'.
+      assert ((dom I ∖ {[n0]}) ∪ {[n0; n1]} ⊆ dom I) as H'.
+      { set_solver. }
+      assert (dom I ⊆ (dom I ∖ {[n0]}) ∪ {[n0; n1]}) as H''.
+      { clear -n0_in_I n1_in_I n0_neq_n1. intros x Hx. 
+        destruct (decide (x = n0)); first by set_solver.
+        destruct (decide (x = n1)); first by set_solver.
+        by set_solver. }
+      set_solver. }  
+    assert ((dom I ∖ {[n0]}) ∩ dom I' = {[n1]}) as H''.
+    { rewrite Dom_I'. set_solver. }
+    assert (rank n0 < rank n1) as Rank_n0_n1.
+    { assert (edgeset es n0 n1 ≠ ∅) as Hes.
+      { admit. } 
+      by pose proof EdgeRank n0 n1 Hes. }
+    assert (∀ x : Node, x ∈ dom I' → rank x ≤ rank n1) as Rank_I0.
+    { rewrite Dom_I'. intros x; rewrite elem_of_union.
+      intros [Hx | Hx].
+      - assert (x = n0) as -> by set_solver.
+        lia.
+      - assert (x = n1) as -> by set_solver.
+        lia. }
+    pose proof flow_upd_defined rank es I k n1 (dom I ∖ {[n0]}) I'
+      EdgeRank ES_I n1_in_I' H' H'' Rank_I0 as Hdef.
+    clear H' H''.
+    destruct (flow_updk_rec es I k n1 (dom I ∖ {[n0]}) I') 
+      as [ (II', nk) |] eqn: Hflow_upd1; try done.
+    assert (∀ x, x ∈ dom I' ∖ {[n1]} → outflow_edge_rel x (es !!! x) (FI I' x)) 
+      as Outflow_I'.
+    { admit. }
+    assert (n0 ∈ dom I') as n0_in_I'.
+    { rewrite Dom_I'. clear; set_solver. }
+    assert (∀ x : Node, x ∈ dom I' ∖ {[n0]} → rank n0 < rank x) as Rank_n0.
+    { intros x. rewrite Dom_I'. rewrite elem_of_difference.
+      rewrite elem_of_union. intros [[Hx1 | Hx1] Hx2]; try done.
+      assert (x = n1) as -> by set_solver. lia. }
+    assert (FI I' n1 = inflow_insert_set (FI I n1) n1 {[k]}) as Def_I'_n.
+    { unfold FI. subst I'. rewrite lookup_total_insert; try done.  }    
+    assert (dom I' ⊆ dom I) as Dom_I'_in_I.
+    { rewrite Dom_I'; clear -n0_in_I n1_in_I; set_solver. }
+    assert (∀ x, x ∈ dom I' ∖ {[n0; n1]} → 
+                  keyset (FI I' x) = keyset (FI I x)) as KS_I'.
+    { rewrite Dom_I'. intros x Hx. clear -Hx; set_solver. }
+    assert (keyset (FI I' n0) = keyset (FI I n0) ∖ {[k]}) as KS_n0.
+    { unfold FI; subst I'. rewrite lookup_total_insert_ne; try done.
+      rewrite lookup_total_insert. subst In0.
+      unfold keyset. rewrite outflow_insert_set_insets.
+      rewrite outflow_insert_set_outsets. clear; set_solver. }  
+    assert (k ∈ insets (FI I n1)) as k_in_Insn1.
+    { admit. }
+    assert (∀ x, x ∈ dom I' → domm (FI I' x) = {[x]}) as Domm_I'.
+    { intros x. rewrite Dom_I'. rewrite elem_of_union.
+      unfold FI; subst I'. intros [Hx | Hx].
+      - assert (x = n0) as -> by (clear -Hx; set_solver).
+        rewrite lookup_total_insert_ne; try done.
+        rewrite lookup_total_insert.
+        subst In0. by apply Domm_I.
+      - assert (x = n1) as -> by (clear -Hx; set_solver).
+        rewrite lookup_total_insert.
+        subst In1. rewrite flowint_inflow_insert_set_dom.
+        rewrite Domm_I; try done. clear; set_solver. }  
+    assert (([^op set] x ∈ dom I', FI I x) = 
+                ([^op set] x ∈ dom I', FI I' x)) as Heq.
+    { admit. }
+    pose proof flow_updk_invariants rank es I k n1 (dom I ∖ {[n0]}) 
+      I' II' nk n0 EdgeRank VI Domm_I ES_I Outflow_I Outflow_I' 
+      n0_in_I' n1_in_I' n0_neq_n1 Rank_I0 Rank_n0 Def_I'_n 
+      Dom_I'_in_I KS_I' KS_n0 k_in_Insn1 Domm_I' Heq Hflow_upd1 
+      as [HInv1 [HInv2 [HInv3 [HInv4 [HInv5 
+            [HInv6 [HInv7 [HInv8 [HInv9 HInv10]]]]]]]]].
+    set III := flow_updk_post I II'.
+    assert (III = flow_updk_post I II') as Def_III.
+    { try done. }
+    assert (dom II' ⊆ dom I) as Dom_II'_in_I.
+    { admit. }
+    pose proof flow_updk_post_summary es k I II' III n0 nk 
+      Dom_II'_in_I HInv8 HInv9 Domm_I HInv10 HInv1 HInv2 HInv3 HInv4 Outflow_I 
+      HInv5 Def_III 
+      as [HInv1' [HInv2' [HInv3' [HInv4' [HInv5' [HInv6' HInv7']]]]]].
+    exists III, nk. repeat split; try done.
+  Admitted.
+
+  Definition add_k (KM: gmap Node (gset K)) (n: Node) (k: K) :=
+    let f := λ s, match s with None => Some {[k]} 
+                            | Some s => Some (s ∪ {[k]}) end in
+    partial_alter f n KM.
+
+  Function flow_upd_rec es n0 I (KM: gmap Node (gset K)) 
+    (A R: gset K) {measure size R} :=
+    match (elements R) with 
+    | [] => Some (I, KM)
+    | k :: _ => 
+      match flow_updk es I k n0 with
+      | Some (I', nk) =>
+        let KM' := add_k KM nk k in
+        flow_upd_rec es n0 I' KM' (A ∪ {[k]}) (R ∖ {[k]})
+      | None => None end end.
+  intros es n0 I KM A R k l HR ? I' nk -> ?.
+  assert (k ∈ R).
+  { apply elem_of_elements. rewrite HR. set_solver. }
+  apply subset_size. set_solver.
+  Defined.
+
+  Definition flow_upd es n0 I0 (S: gset K) :=
+    flow_upd_rec es n0 I0 ∅ ∅ S.
+
+  Lemma flow_upd_invariants rank es n0 I KM A R I' KM' I0:
+    let FI := λ I x, I !!! x in
+    (edge_rank_rel es rank) →
+    (∀ n1 n2, edgeset es n1 n2 ≠ ∅ → n2 ∈ dom I) →
+    (✓ ([^op set] x ∈ dom I, FI I x)) →
+    (∀ x, x ∈ dom I → domm (FI I x) = {[x]}) →
+    (∀ x, x ∈ dom I → outflow_edge_rel x (es !!! x) (FI I x)) →
+    (n0 ∈ dom I) →
+    (∀ k, k ∈ R → find_next (es !!! n0) k ≠ None) →
+    (([^op set] x ∈ dom I, FI I0 x) = ([^op set] x ∈ dom I, FI I x)) →
+    (keyset (FI I n0) = keyset (FI I0 n0) ∖ A) →
+    flow_upd_rec es n0 I KM A R = Some (I', KM') →
+        (([^op set] x ∈ dom I, FI I0 x) = ([^op set] x ∈ dom I, FI I' x)
+      ∧ (keyset (FI I' n0) = keyset (FI I0 n0) ∖ (A ∪ R))).
+  Proof.
+    intros FI. apply flow_upd_rec_ind; try done.
+    - clear I KM A R. intros I KM A R HR EdgeRank ES_I VI Domm_I Outflow_I 
+        n0_in_I FN_n0 Heq KS_n0 [= -> ->]. split; try done.
+        assert (R = ∅) as ->.
+        { apply leibniz_equiv. by apply elements_empty_inv. }
+        by rewrite union_empty_r_L. 
+    - clear I KM A R. intros I KM A R k ks HR II nk Hflowk KMM HInd. 
+      intros EdgeRank ES_I VI Domm_I Outflow_I n0_in_I FN_n0 Heq KS_n0 Hflow.
+      assert (k ∈ R) as k_in_R.
+      { apply elem_of_elements. rewrite HR. clear; set_solver. }
+      assert (find_next (es !!! n0) k ≠ None) as FN_n0_k.
+      { apply FN_n0; try done. } 
+      pose proof flow_updk_summary rank es I k n0 (Some (II, nk))
+        EdgeRank ES_I VI Domm_I Outflow_I n0_in_I FN_n0_k Hflowk 
+        as [? [? [[= <- <-] Hsum]]].
+      destruct Hsum as [HInv1 [HInv2 [HInv3 [HInv4 
+              [HInv5 [HInv6 [HInv7 HInv8]]]]]]].
+      assert (([^op set] x ∈ dom I, FI I0 x) =
+                ([^op set] x ∈ dom I, FI II x)) as Heq'.
+      { rewrite Heq. by unfold FI. }          
+      rewrite HInv1 in HInd.
+      assert (A ∪ {[k]} ∪ R ∖ {[k]} = A ∪ R) as H'.
+      { admit. }
+      rewrite H' in HInd.
+      apply HInd; try done; clear HInd.
+      + by rewrite <-Heq'; rewrite Heq.
+      + by rewrite <-HInv1.
+      + intros k' Hk'. apply FN_n0.
+        clear -Hk'; set_solver.
+      + unfold FI. rewrite HInv6.
+        rewrite KS_n0. unfold FI.
+        clear; set_solver.      
+
+
+  Admitted.    
+      
     
+
+End list_flow_upd.    
